move thread specs to [thread/spec.v], fix [custom_mutex_hpp_proof.v]

rocq-brick-libstdcpp/proof/thread/thread.hpp
@@ -1,1 +1,4 @@
 #include <thread>
+
+template std::thread::thread(void (*&)());
+template std::thread::thread(void (&)());
