rocq-brick-libstdcpp/test/mutex/custom_mutex_hpp_proof.v
@@ -9,58 +9,69 @@ Require Import skylabs.brick.libstdcpp.mutex.requirements.
 Require Import skylabs.brick.libstdcpp.lib.lock_ghost2.
 Require Import skylabs.brick.libstdcpp.atomic.spec.
 Require Import skylabs.brick.libstdcpp.cassert.spec.
+Require Import skylabs.brick.libstdcpp.thread.spec.
 Import linearity.
 Require Import skylabs.brick.libstdcpp.test.mutex.custom_mutex_hpp.
 
-(** The ghost implementation and its physical client predicates are specific
-    to [MyMutex]. The entire mutex-set pool still uses one shared ghost name. *)
-Module CustomMutexState (Sets0 : MUTEX_SETS) (Tokens0 : MUTEX_TOKENS)
-    (Owners0 : OWNER_TID) <: MUTEX_PREDS.
-  Record mutex_gname : Set := MkGname {
+(** The concrete mutex supplies both the ghost state and the physical
+    predicates used by [mutex_spec]. The mutex-set pool is shared, and the
+    memory-order global remains a separate precondition of the C++ methods. *)
+Module CustomMutexPreds <: MUTEX_PREDS.
+  Import MutexSets MutexTokens OwnerTid.
+
+  Record state_gname : Set := MkStateGname {
     pool_gname : iprop.gname;
     token_gname : iprop.gname;
     owner_gname : iprop.gname;
   }.
+
+  Definition class_name : name := "MyMutex"%cpp_name.
+  Definition cpp_ty : type := Tnamed class_name.
+  Record mutex_gname : Set := MkGname {
+    lock_state_gname :> state_gname;
+    cinv_gname : iprop.gname;
+  }.
   Definition gname : Set := mutex_gname.
-  Definition pool_name (γ : gname) : iprop.gname := γ.(pool_gname).
+  Definition pool_name (γ : gname) : iprop.gname :=
+    γ.(lock_state_gname).(pool_gname).
 
   Definition mutex_inv_namespace : namespace :=
     nroot .@@ "MyMutex" .@ "inv_namespace".
 
   Class stateG `{Σ : cpp_logic} := {
-    #[global] sets_G :: Sets0.G Σ;
-    #[global] tokens_G :: Tokens0.G Σ;
-    #[global] owners_G :: Owners0.G Σ;
+    #[global] sets_G :: MutexSets.G Σ;
+    #[global] tokens_G :: MutexTokens.G Σ;
+    #[global] owners_G :: OwnerTid.G Σ;
   }.
   Definition G := @stateG.
   Existing Class G.
   #[global] Arguments G {_ _} Σ : assert.
   #[global] Instance state_G `{Σ : cpp_logic} (H : G Σ) : @stateG _ _ Σ := H.
 
-  Definition token `{Σ : cpp_logic, !G Σ}
-      (γ : gname) (q : cQp.t) : mpred :=
-    Tokens0.token γ.(token_gname) q.
+  Definition state_token `{Σ : cpp_logic, !G Σ}
+      (γ : state_gname) (q : cQp.t) : mpred :=
+    MutexTokens.token γ.(token_gname) q.
 
   Definition not_locked_ghost `{Σ : cpp_logic, !G Σ}
-      (γ : mutex_gname) (th : thread_idT) (q : Qp) : mpred :=
-    Sets0.my_mutexes γ.(pool_gname) th (coPset.CoPset $ ↑mutex_inv_namespace) **
-    Tokens0.token γ.(token_gname) q.
+      (γ : state_gname) (th : thread_idT) (q : Qp) : mpred :=
+    MutexSets.my_mutexes γ.(pool_gname) th (coPset.CoPset $ ↑mutex_inv_namespace) **
+    MutexTokens.token γ.(token_gname) q.
 
   Definition owner_token `{Σ : cpp_logic, !G Σ}
-      (γ : mutex_gname) (th : thread_idT) (q : Qp) : mpred :=
-    Tokens0.given_token γ.(token_gname) q **
-    Owners0.owner_tid_frag γ.(owner_gname) (Some th).
+      (γ : state_gname) (th : thread_idT) (q : Qp) : mpred :=
+    MutexTokens.given_token γ.(token_gname) q **
+    OwnerTid.owner_tid_frag γ.(owner_gname) (Some th).
 
-  #[global] Instance token_fractional
-      `{Σ : cpp_logic, !G Σ} γ : CFractional (token γ).
+  #[global] Instance state_token_fractional
+      `{Σ : cpp_logic, !G Σ} γ : CFractional (state_token γ).
   Proof.
-    intros q1 q2. rewrite /token cQp.frac_add.
-    apply Tokens0.token_fractional.
+    intros q1 q2. rewrite /state_token cQp.frac_add.
+    apply MutexTokens.token_fractional.
   Qed.
 
-  #[global] Instance token_timeless
-      `{Σ : cpp_logic, !G Σ} γ q : Timeless (token γ q).
-  Proof. rewrite /token. apply _. Qed.
+  #[global] Instance state_token_timeless
+      `{Σ : cpp_logic, !G Σ} γ q : Timeless (state_token γ q).
+  Proof. rewrite /state_token. apply _. Qed.
 
   #[global] Instance owner_token_timeless
       `{Σ : cpp_logic, !G Σ} γ th q : Timeless (owner_token γ th q).
@@ -77,15 +88,15 @@ Module CustomMutexState (Sets0 : MUTEX_SETS) (Tokens0 : MUTEX_TOKENS)
       and the token balance. The thread retains its remaining mutex names.
       When free, both halves of the previous owner remain in the invariant. *)
   Definition state `{Σ : cpp_logic, !G Σ}
-      (γ : mutex_gname) (b : bool) : mpred :=
+      (γ : state_gname) (b : bool) : mpred :=
     (if b then
-      ∃ th, Owners0.owner_tid_auth γ.(owner_gname) (Some th) **
-        Sets0.my_mutexes γ.(pool_gname) th (coPset.CoPset $ ↑mutex_inv_namespace) **
-        Tokens0.token_not_full γ.(token_gname)
+      ∃ th, OwnerTid.owner_tid_auth γ.(owner_gname) (Some th) **
+        MutexSets.my_mutexes γ.(pool_gname) th (coPset.CoPset $ ↑mutex_inv_namespace) **
+        MutexTokens.token_not_full γ.(token_gname)
     else
-      ∃ owner, Owners0.owner_tid_auth γ.(owner_gname) owner **
-        Owners0.owner_tid_frag γ.(owner_gname) owner **
-        Tokens0.token_full γ.(token_gname))%I.
+      ∃ owner, OwnerTid.owner_tid_auth γ.(owner_gname) owner **
+        OwnerTid.owner_tid_frag γ.(owner_gname) owner **
+        MutexTokens.token_full γ.(token_gname))%I.
 
   #[global] Instance state_WeaklyObjective
       `{Σ : cpp_logic, !G Σ} γ b :
@@ -95,33 +106,33 @@ Module CustomMutexState (Sets0 : MUTEX_SETS) (Tokens0 : MUTEX_TOKENS)
   Section state_laws.
     Context `{Σ : cpp_logic, !G Σ}.
 
-    Lemma alloc (γpool : iprop.gname) :
+    Lemma alloc_state (γpool : iprop.gname) :
       ⊢ |==> ∃ γ, [| γ.(pool_gname) = γpool |] **
-        token γ 1$m ** state γ false.
+        state_token γ 1$m ** state γ false.
     Proof.
-      iMod Tokens0.alloc as (gt) "[T GT]".
-      iMod (Owners0.alloc None) as (go) "[OA OF]".
-      iModIntro. iExists (MkGname γpool gt go).
+      iMod MutexTokens.alloc as (gt) "[T GT]".
+      iMod (OwnerTid.alloc None) as (go) "[OA OF]".
+      iModIntro. iExists (MkStateGname γpool gt go).
       iSplit; first done.
-      rewrite /token /state /=. iFrame "T". iExists None.
+      rewrite /state_token /state /=. iFrame "T". iExists None.
       iFrame "OA OF".
-      iApply Tokens0.token_full_init. iExact "GT".
+      iApply MutexTokens.token_full_init. iExact "GT".
     Qed.
 
-    Lemma do_lock γ th q :
+    Lemma state_lock γ th q :
       state γ false ** not_locked_ghost γ th q |--
         (|==> state γ true ** owner_token γ th q).
     Proof.
       rewrite /state /not_locked_ghost /owner_token.
       iIntros "[State [Sets T]]".
       iDestruct "State" as (owner) "(OA & OF & Balance)".
-      iDestruct (Tokens0.acquire with "[$Balance $T]") as "[GT Balance]".
-      iMod (Owners0.owner_update γ.(owner_gname) _ _ (Some th)
+      iDestruct (MutexTokens.acquire with "[$Balance $T]") as "[GT Balance]".
+      iMod (OwnerTid.owner_update γ.(owner_gname) _ _ (Some th)
         with "[$OA $OF]") as "[OA OF]".
       iModIntro. iFrame "GT OF". iExists th. iFrame.
     Qed.
 
-    Lemma do_unlock γ th q :
+    Lemma state_unlock γ th q :
       state γ true ** owner_token γ th q |--
         (|==> state γ false ** not_locked_ghost γ th q).
     Proof.
@@ -130,7 +141,7 @@ Module CustomMutexState (Sets0 : MUTEX_SETS) (Tokens0 : MUTEX_TOKENS)
       iDestruct "State" as (owner) "(OA & Sets & Balance)".
       iDestruct (observe_2 [| Some owner = Some th |] with "OA OF") as %Heq.
       injection Heq as ->.
-      iDestruct (Tokens0.release with "[$Balance $GT]") as "[T Balance]".
+      iDestruct (MutexTokens.release with "[$Balance $GT]") as "[T Balance]".
       iModIntro. iFrame "Sets T". iExists (Some th). iFrame.
     Qed.
 
@@ -139,224 +150,261 @@ Module CustomMutexState (Sets0 : MUTEX_SETS) (Tokens0 : MUTEX_TOKENS)
     Proof.
       rewrite /state /owner_token. iIntros "[State [_ OF]]".
       iDestruct "State" as (owner) "(_ & OF0 & _)".
-      iDestruct (Owners0.owner_tid_frag_exclusive with "OF0 OF") as %[].
+      iDestruct (OwnerTid.owner_tid_frag_exclusive with "OF0 OF") as %[].
     Qed.
 
     Lemma locked_full_token γ :
-      state γ true ** token γ 1$m |-- False.
+      state γ true ** state_token γ 1$m |-- False.
     Proof.
-      rewrite /state /token. iIntros "[State T]".
+      rewrite /state /state_token. iIntros "[State T]".
       iDestruct "State" as (th) "(_ & _ & Balance)".
-      iApply (Tokens0.token_not_full_full_token with "[$Balance $T]").
+      iApply (MutexTokens.token_not_full_full_token with "[$Balance $T]").
     Qed.
   End state_laws.
 
-  #[global] Hint Opaque token not_locked_ghost owner_token state : sl_opacity typeclass_instances.
-
-  Parameter thread_idR : ∀ `{Σ : cpp_logic, σ : genv}, cQp.t ->
-    (* None if value is thread::id(), Some otherwise *)
-    option thread_idT -> Rep.
-  #[only(cfracsplittable, type_ptr="std::thread::id")] derive thread_idR.
-  #[global] Axiom thread_idR_WeaklyObjective :
-    ∀ `{Σ : cpp_logic, σ : genv} (q : cQp.t)
-      (o : option thread_idT) (p : ptr),
-      WeaklyObjective (thread_idR q o p).
-  #[global] Existing Instance thread_idR_WeaklyObjective.
+  #[global] Hint Opaque state_token not_locked_ghost owner_token state : sl_opacity typeclass_instances.
 
   Definition globals `{Σ : cpp_logic} {σ : genv} (q : cQp.t) : mpred :=
     _global "std::memory_order_seq_cst" |->
       primR "enum std::memory_order" q
         (memory_order.to_val memory_order.seq_cst).
 
-  Definition not_locked `{Σ : cpp_logic, !G Σ} {σ : genv}
-      (this : ptr) (γ : gname) (th : thread_idT) (q : cQp.t) : mpred :=
-    not_locked_ghost γ th q ** globals q.
-  #[global] Arguments not_locked /.
   #[global] Arguments globals /.
 
+  Definition token `{Σ : cpp_logic, !G Σ} (γ : gname) (q : cQp.t) : mpred :=
+    state_token γ q.
+  Definition not_locked `{Σ : cpp_logic, !G Σ} {σ : genv}
+      (this : ptr) (γ : gname) (th : thread_idT) (q : cQp.t) : mpred :=
+    not_locked_ghost γ th q.
+  Definition locked `{Σ : cpp_logic, !G Σ} {σ : genv}
+      (this : ptr) (γ : gname) (th : thread_idT) (q : cQp.t) : mpred :=
+    this ,, _field "MyMutex::m_owner" |-> thread_idR 1$m (Some th) **
+      owner_token γ th q.
+  #[global] Hint Opaque token : sl_opacity typeclass_instances.
+  #[global] Hint Opaque locked : typeclass_instances.
+  #[global] Arguments not_locked /.
+  #[global] Arguments locked /.
+
+  #[global] Instance token_fractional `{Σ : cpp_logic, !G Σ} γ :
+      CFractional (token γ).
+  Proof. rewrite /token. apply state_token_fractional. Qed.
+  #[global] Instance token_timeless `{Σ : cpp_logic, !G Σ} γ q :
+      Timeless (token γ q).
+  Proof. rewrite /token. apply _. Qed.
   #[global] Instance not_locked_timeless `{Σ : cpp_logic, !G Σ} {σ : genv}
       this γ th q : Timeless (not_locked this γ th q).
-  Proof. rewrite /not_locked /not_locked_ghost /globals. apply _. Qed.
+  Proof. rewrite /not_locked /not_locked_ghost. apply _. Qed.
   #[global] Instance not_locked_exclusive `{Σ : cpp_logic, !G Σ} {σ : genv}
       this γ th : Exclusive1 (not_locked this γ th).
   Proof.
     intros q1 q2. rewrite /not_locked /not_locked_ghost.
-    iIntros "[[F1 _] _] [[F2 _] _]".
+    iIntros "[F1 _] [F2 _]".
     have Hnonempty : (↑ mutex_inv_namespace : coPset) ∩ ↑ mutex_inv_namespace ≠ ∅.
     { rewrite intersection_idemp_L. apply nclose_non_empty. }
-    iDestruct (Sets0.my_mutexes_exclusive γ.(pool_gname) th
+    iDestruct (MutexSets.my_mutexes_exclusive _ th
       (↑ mutex_inv_namespace) (↑ mutex_inv_namespace) Hnonempty
       with "[$F1 $F2]") as %[].
   Qed.
-
-  (** Public ownership includes the physical owner written by [lock]. *)
-  Definition locked `{Σ : cpp_logic, !G Σ} {σ : genv}
-      (this : ptr) (γ : gname) (th : thread_idT) (q : cQp.t) : mpred :=
-    globals q **
-      (this ,, _field "MyMutex::m_owner" |-> thread_idR 1$m (Some th) **
-        owner_token γ th q).
-  #[global] Arguments locked /.
   #[global] Instance locked_timeless `{Σ : cpp_logic, !G Σ} {σ : genv}
       this γ th q : Timeless (locked this γ th q).
-  Proof. rewrite /locked /globals. apply _. Qed.
+  Proof. rewrite /locked. apply _. Qed.
   #[global] Instance locked_exclusive `{Σ : cpp_logic, !G Σ} {σ : genv}
       this γ : Exclusive2 (locked this γ).
-  Proof.
-    intros th1 th2 q1 q2. rewrite /locked.
-    apply observe_2_sep_r. apply observe_2_sep_r. apply _.
-  Qed.
-
-End CustomMutexState.
-
-Module LockState := CustomMutexState MutexSets MutexTokens OwnerTid.
-
-(** Verify the implementation using its ghost resources and public state predicates. *)
-Module custom_mutex.
-  Module State := LockState.
-  Module Spec := mutex_spec State.
-
-  Abbreviation N := "MyMutex"%cpp_name.
-  Abbreviation thread_idR := LockState.thread_idR.
-  #[local] Hint Opaque LockState.thread_idR : sl_opacity typeclass_instances.
+  Proof. intros th1 th2 q1 q2. rewrite /locked. apply observe_2_sep_r. apply _. Qed.
 
   #[local] Instance at_WeaklyObjective `{Σ : cpp_logic}
       (p : ptr) (R : Rep) `{!WeaklyObjective (R p)} :
     WeaklyObjective (p |-> R).
   Proof. rewrite INTERNAL._at_eq. apply _. Qed.
 
-  (* thread::id operations and yield() are not proved for now. *)
-  Section unproved_specs.
-    Context `{Σ : cpp_logic, σ : genv, HAS_THREADS : !HasStdThreads Σ}.
-    Context `{MOD : source ⊧ σ}.
-
-    cpp.spec (default_ctor "std::thread::id") as thread_id_ctor_spec with (
-      \this this
-      \post this |-> thread_idR 1$m None).
-
-    cpp.spec (const_copy_ctor "std::thread::id") as thread_id_copy_ctor_spec with (
-      \this this
-      \arg{other} "" (Vptr other)
-      \prepost{q o} other |-> thread_idR q o
-      \post this |-> thread_idR 1$m o).
-
-    cpp.spec (dtor "std::thread::id") as thread_id_dtor_spec with (
-      \this this
-      \pre{o} this |-> thread_idR 1$m o
-      \post emp).
-
-    cpp.spec "std::thread::id::operator=(const std::thread::id&)"
-        as thread_id_copy_assign_spec with (
-      \this this
-      \arg{other} "" (Vptr other)
-      \pre{old} this |-> thread_idR 1$m old
-      \prepost{q o} other |-> thread_idR q o
-      \post[Vref this] this |-> thread_idR 1$m o).
-
-    cpp.spec "std::thread::id::operator=(std::thread::id&&)"
-        as thread_id_move_assign_spec with (
-      \this this
-      \arg{other} "" (Vptr other)
-      \pre{old} this |-> thread_idR 1$m old
-      \prepost{o} other |-> thread_idR 1$m o
-      \post[Vref this] this |-> thread_idR 1$m o).
-
-    cpp.spec "std::operator==(std::thread::id, std::thread::id)"
-        as thread_id_eq_spec with (
-      \arg{lhs} "" (Vptr lhs)
-      \arg{rhs} "" (Vptr rhs)
-      \prepost{q1 o1} lhs |-> thread_idR q1 o1
-      \prepost{q2 o2} rhs |-> thread_idR q2 o2
-      \post[Vbool (bool_decide (o1 = o2))] emp).
-
-    cpp.spec "std::this_thread::get_id()" as get_id_spec with (
-      \persist{thr} current_thread thr
-      \post{result}[Vptr result]
-        result |-> thread_idR 1$m (Some thr)).
-
-    cpp.spec "std::this_thread::yield()" as yield_spec with (
-      \post emp).
-  End unproved_specs.
-
-  Record gname : Set := MkGname {
-    lock_state_gname :> State.mutex_gname;
-    cinv_gname : iprop.gname;
-  }.
-
   Section with_Σ.
-    Context `{Σ : cpp_logic, σ : genv, HAS_THREADS : !HasStdThreads Σ,
-      !State.G Σ}.
+    Context `{Σ : cpp_logic, !G Σ}.
 
     (** The physical lock bit agrees with the abstract ghost state. The
         protected resources and cleared owner field are available while free. *)
-    Definition mutex_inv (this : ptr) (γ : gname) (P : mpred) : mpred :=
+    Definition mutex_inv {σ : genv} (this : ptr) (γ : gname) (P : mpred) : mpred :=
       ∃ b : bool,
       this ,, _field "MyMutex::m_lock" |->
         atomic.R "int" 1$m (if b then 1 else 0)%Z **
-      State.state γ b **
+      state γ b **
       if b then emp else
         P ** this ,, _field "MyMutex::m_owner" |-> thread_idR 1$m None.
 
-    Definition IR (γ : gname) (q : cQp.t) (P : mpred) : Rep :=
-      structR N q$m **
+    Definition R {HAS_THREADS : HasStdThreads Σ} {σ : genv} (γ : gname) (q : cQp.t) (P : mpred) : Rep :=
+      structR class_name q$m **
       as_Rep (fun this =>
-        cinv State.mutex_inv_namespace (cinv_gname γ) (mutex_inv this γ P) **
+        cinv mutex_inv_namespace (cinv_gname γ) (mutex_inv this γ P) **
         cinv_own (cinv_gname γ) q
       ).
-    Hint Opaque IR : sl_opacity typeclass_instances.
-    #[only(type_ptr,cfractional,ascfractional,cfracvalid)] derive IR.
+    #[global] Hint Opaque R : sl_opacity typeclass_instances.
+    #[only(type_ptr,cfractional,ascfractional,cfracvalid)] derive R.
+
+    #[global] Instance R_learnable {HAS_THREADS : HasStdThreads Σ} {σ : genv} :
+      Cbn (Learn (learn_eq ==> any ==> learn_eq ==> learn_hints.fin) R).
+    Proof. solve_learnable. Qed.
+
+    Context {σ : genv} {HAS_THREADS : HasStdThreads Σ}.
+
+    #[global] Instance locked_learn :
+        Cbn (Learn (req_eq ==> learn_eq ==> req_eq ==> req_eq ==> learn_hints.fin) locked).
+    Proof. solve_learnable. Qed.
+
+    Definition do_lock (this : ptr) (lk : gname * mpred) (K : mpred) : mpred :=
+      ∃ thr qt, current_thread thr ** not_locked this lk.1 thr qt **
+        (locked this lk.1 thr qt ** lk.2 -* K).
+    #[global] Arguments do_lock /.
+
+    Definition do_unlock (this : ptr) (lk : gname * mpred) (K : mpred) : mpred :=
+      ∃ thr qt, current_thread thr ** locked this lk.1 thr qt ** ▷lk.2 **
+        (not_locked this lk.1 thr qt -* K).
+    #[global] Arguments do_unlock /.
+
+    #[global] Instance mutex_basic_lockable :
+        BasicLockable (T := gname * mpred) cpp_ty
+          (fun q gP => R gP.1 q gP.2) :=
+      { do_lock := do_lock
+      ; do_unlock := do_unlock }.
+
+    Definition do_try_lock (this : ptr) (lk : gname * mpred)
+        (K : bool -> mpred) : mpred :=
+      ∃ thr qt, current_thread thr ** not_locked this lk.1 thr qt **
+        ∀ b : bool,
+          (if b then lk.2 ** locked this lk.1 thr qt
+            else not_locked this lk.1 thr qt) -* K b.
+    #[global] Arguments do_try_lock /.
+
+    #[global] Instance mutex_lockable :
+        Lockable (T := gname * mpred) cpp_ty
+          (fun q gP => R gP.1 q gP.2) :=
+      { do_try_lock := do_try_lock }.
+
+    Lemma init_R (this : ptr) (old : gname)
+        (pool : iprop.gname) (P : mpred) :
+      WeaklyObjective P ->
+      this |-> R old 1$m emp ** token old 1$m ** ▷P |--
+        (|={⊤}=> ∃ g, this |-> R g 1$m P ** token g 1$m).
+    Proof.
+      intros HP. iIntros "(HR & T & P)".
+      iEval (rewrite /R _at_sep _at_as_Rep) in "HR".
+      iDestruct "HR" as "(S & #CI & CO)".
+      iMod (cinv_cancel with "CI CO") as "Inv"; [done..|].
+      iMod (alloc_state pool) as (gs) "(_ & Tnew & Stnew)".
+      iMod (cinv_alloc with "[Inv P Stnew T]") as (gi) "[#CInew COnew]"; last first.
+      - iModIntro. iExists (MkGname gs gi).
+        rewrite /R _at_sep _at_as_Rep /token /mutex_inv /=.
+        iFrame "CInew S COnew Tnew".
+      - iNext. rewrite /mutex_inv.
+        iDestruct "Inv" as (b) "(L & St & Resources)".
+        destruct b.
+        + iDestruct (locked_full_token with "[$St $T]") as %[].
+        + iDestruct "Resources" as "[_ Owner]".
+          iExists false. iFrame "L Stnew P Owner".
+          iApply (affine with "[St T]"); last iAccu. apply mpred_BiAffine.
+      - apply _.
+    Qed.
+
+    Lemma register_thread
+        (this : ptr) (g : gname) (q : cQp.t) (P : mpred)
+        (th : thread_idT) (qt : cQp.t) :
+      this |-> R g q P ** token g qt **
+      MutexSets.my_mutexes (pool_name g) th
+        (coPset.CoPset $ ↑mutex_inv_namespace) |--
+      this |-> R g q P ** not_locked this g th qt.
+    Proof.
+      rewrite /not_locked /not_locked_ghost /token /state_token /pool_name.
+      iIntros "($ & T & M)". iFrame.
+    Qed.
+  End with_Σ.
+End CustomMutexPreds.
+
+(** Verify the implementation using its ghost resources and public state predicates. *)
+Module custom_mutex.
+  Import CustomMutexPreds.
+  Module Spec := mutex_spec CustomMutexPreds.
+
+  Abbreviation N := "MyMutex"%cpp_name.
+  #[local] Hint Opaque thread_idR : sl_opacity typeclass_instances.
+
+  #[local] Instance at_WeaklyObjective `{Σ : cpp_logic}
+      (p : ptr) (R : Rep) `{!WeaklyObjective (R p)} :
+    WeaklyObjective (p |-> R).
+  Proof. rewrite INTERNAL._at_eq. apply _. Qed.
+
+  Abbreviation IR := CustomMutexPreds.R.
+
+  Section with_Σ.
+    Context `{Σ : cpp_logic, σ : genv, HAS_THREADS : !HasStdThreads Σ,
+      !CustomMutexPreds.G Σ}.
 
     Context `{MOD : source ⊧ σ}.
 
+    (* FIXME any reason to keep Reduce? *)
     cpp.spec "MyMutex::MyMutex()" as ctor_spec with
-      (\exact Reduce (Spec.ctor_spec IR lock_state_gname)).
+      (\exact Reduce (Spec.ctor_spec)).
 
     cpp.spec "MyMutex::~MyMutex()" as dtor_spec with
-      (\exact Reduce (Spec.dtor_spec IR lock_state_gname)).
+      (\exact Reduce (Spec.dtor_spec)).
 
     Definition T : Type := gname * mpred.
     cpp.spec "MyMutex::do_lock()" as do_lock_spec with (
       \this this
       \prepost{g q P} this |-> IR g q P
       \persist{thr} current_thread thr
-      \pre{(qt : cQp.t)} State.not_locked_ghost g thr qt ** State.globals qt
-      \post P ** State.globals qt **
+      \prepost{qg} globals qg
+      \pre{(qt : Qp)} not_locked_ghost g thr qt
+      \post P **
         this ,, _field "MyMutex::m_owner" |-> thread_idR 1$m None **
-        State.owner_token g thr qt).
+        owner_token g thr qt).
 
     cpp.spec "MyMutex::do_unlock()" as do_unlock_spec with (
       \this this
       \prepost{g q P} this |-> IR g q P
       \persist{thr} current_thread thr
-      \pre{qt} State.globals qt **
-        this ,, _field "MyMutex::m_owner" |-> thread_idR 1$m None **
-        State.owner_token g thr qt
+      \prepost{qg} globals qg
+      \pre{qt} this ,, _field "MyMutex::m_owner" |-> thread_idR 1$m None **
+        owner_token g thr qt
       \pre ▷P
-      \post State.not_locked_ghost g thr qt ** State.globals qt).
-
-    Definition do_lock := Spec.do_lock lock_state_gname.
-    #[global] Arguments do_lock /.
-    Definition do_unlock := Spec.do_unlock lock_state_gname.
-    #[global] Arguments do_unlock /.
-
-    #[global] Instance custom_mutex_basic_lockable :
-        BasicLockable (T := T) (Tnamed N)
-          (fun q gP => IR gP.1 q gP.2) :=
-      { do_lock := do_lock
-      ; do_unlock := do_unlock }.
+      \post not_locked_ghost g thr qt).
 
     cpp.spec "MyMutex::lock()" as lock_spec_alt with
-      (\exact Reduce (Spec.lock_spec_alt IR lock_state_gname)).
+      (\this this
+       \prepost{qg} globals qg
+       \exact Reduce (Spec.lock_spec_alt this)).
 
     cpp.spec "MyMutex::unlock()" as unlock_spec_alt with
-      (\exact Reduce (Spec.unlock_spec_alt IR lock_state_gname)).
+      (\this this
+       \prepost{qg} globals qg
+       \exact Reduce (Spec.unlock_spec_alt this)).
 
     cpp.spec "MyMutex::lock()" as lock_spec with
-      (\exact Reduce
-        (lock_basic_lockable (Tnamed N) (fun q gP => IR gP.1 q gP.2))).
+      (\this this
+       \prepost{qg} globals qg
+       \exact Reduce
+        (Spec.lock_spec this)).
 
     cpp.spec "MyMutex::unlock()" as unlock_spec with
-      (\exact Reduce
-        (unlock_basic_lockable (Tnamed N) (fun q gP => IR gP.1 q gP.2))).
+      (\this this
+       \prepost{qg} globals qg
+       \exact Reduce
+        (Spec.unlock_spec this)).
+
+    Lemma lock_spec_equiv_lock_spec_alt : lock_spec ⊣⊢ lock_spec_alt.
+    Proof.
+      rewrite /lock_spec /lock_spec_alt /specify.
+      do 2 f_equiv. intros this xs K.
+      rewrite !add_with_equiv.
+      f_equiv=> qg.
+      by rewrite !add_prepost_equiv Spec.lock_spec_equiv_lock_spec_alt.
+    Qed.
+
+    Lemma unlock_spec_equiv_unlock_spec_alt : unlock_spec ⊣⊢ unlock_spec_alt.
+    Proof.
+      rewrite /unlock_spec /unlock_spec_alt /specify.
+      do 2 f_equiv. intros this xs K.
+      rewrite !add_with_equiv.
+      f_equiv=> qg.
+      by rewrite !add_prepost_equiv Spec.unlock_spec_equiv_unlock_spec_alt.
+    Qed.
 
     Abbreviation BASE p := (p ,, _base "std::atomic<int>" "std::__atomic_base<int>").
 
@@ -370,13 +418,13 @@ Module custom_mutex.
       \using denoteModule source
       \using{thr} current_thread thr
       \consuming{g q P} p |-> IR g q P
-      \consuming{qt} State.not_locked_ghost g thr qt
+      \consuming{qt} not_locked_ghost g thr qt
       \proving{K (_ : IsExistential K)}
       std.atomic.do_exchange "int" (BASE (p,, o_field σ "MyMutex::m_lock") ) 1%Z K
       \instantiate K := (fun res => p |-> IR g q P ** [| res = 0 \/ res = 1 |]%Z **
-                          if bool_decide (res = 0) then P ** State.owner_token g thr qt **
+                          if bool_decide (res = 0) then P ** owner_token g thr qt **
                             p ,, _field "MyMutex::m_owner" |-> thread_idR 1$m None
-                          else State.not_locked_ghost g thr qt)
+                          else not_locked_ghost g thr qt)
                           \end@{mpredI}.
     Next Obligation.
       intros. iIntros "[#M Hpre]" (?? ->).
@@ -386,7 +434,7 @@ Module custom_mutex.
       iDestruct "IR" as "(S & #CI & CO)".
       rewrite /std.atomic.do_exchange.
       iAuIntro1. rewrite /atomic1_acc.
-      iInv State.mutex_inv_namespace as "Inv" "Hclose".
+      iInv mutex_inv_namespace as "Inv" "Hclose".
       iDestruct "Inv" as "[Inv CO]".
       iEval (rewrite /mutex_inv) in "Inv".
       iDestruct "Inv" as (b) "(>L & State & Resources)".
@@ -410,7 +458,7 @@ Module custom_mutex.
           iModIntro. rewrite /IR _at_sep _at_as_Rep /=.
           iFrame "CI". iFrame. iPureIntro. auto.
         + iDestruct "Resources" as "[P Owner]".
-          iMod (State.do_lock _ with "[$State $NL]") as "[State Locked]".
+          iMod (state_lock _ with "[$State $NL]") as "[State Locked]".
           iMod ("Hclose" with "[L State]") as "_".
           { iNext. rewrite /mutex_inv. iExists true.
             iSplitL "L"; first by ework $usenamed=true with br_erefl.
@@ -428,10 +476,10 @@ Module custom_mutex.
       \consuming{g q P} p |-> IR g q P
       \consuming P
       \consuming p ,, _field "MyMutex::m_owner" |-> thread_idR 1$m None
-      \consuming{qt} State.owner_token g thr qt
+      \consuming{qt} owner_token g thr qt
       \proving{K (_ : IsExistential K)}
         std.atomic.do_store "int" (BASE (p ,, o_field σ "MyMutex::m_lock")) 0%Z K
-      \instantiate K := (p |-> IR g q P ** State.not_locked_ghost g thr qt)
+      \instantiate K := (p |-> IR g q P ** not_locked_ghost g thr qt)
       \end@{mpredI}.
     Next Obligation.
       intros. iIntros "[#M Hpre]" (?? ->).
@@ -441,7 +489,7 @@ Module custom_mutex.
       iDestruct "IR" as "(S & #CI & CO)".
       rewrite /std.atomic.do_store.
       iAcIntro. rewrite /commit_acc /=.
-      iInv State.mutex_inv_namespace as "Inv" "Hclose".
+      iInv mutex_inv_namespace as "Inv" "Hclose".
       iDestruct "Inv" as "[Inv CO]".
       iEval (rewrite /mutex_inv) in "Inv".
       iDestruct "Inv" as (b) "(>L & State & Resources)".
@@ -450,7 +498,7 @@ Module custom_mutex.
       iSplitL "L"; first by ework $usenamed=true with br_erefl.
       iNext. iIntros "L". iMod "Y" as "_".
       destruct b.
-      - iMod (State.do_unlock _ with "[$State $Locked]") as "[State NL]".
+      - iMod (state_unlock _ with "[$State $Locked]") as "[State NL]".
         iMod ("Hclose" with "[L State P Owner]") as "_".
         { iNext. rewrite /mutex_inv. iExists false.
           iSplitL "L"; first by ework $usenamed=true with br_erefl.
@@ -458,7 +506,7 @@ Module custom_mutex.
         iModIntro.
         rewrite /IR _at_sep _at_as_Rep /=.
         iFrame "CI". iFrame.
-      - iDestruct (State.unlocked_owner_token with "[$State $Locked]") as %[].
+      - iDestruct (unlocked_owner_token with "[$State $Locked]") as %[].
     Qed.
     Hint Resolve do_store_C : sl_opacity.
 
@@ -496,9 +544,13 @@ Module custom_mutex.
       verify_spec; go.
     Qed.
 
+    #[local] Remove Hints CustomMutexPreds.locked_learn : typeclass_instances.
+
     Lemma mymutex_lock_alt_proof : verify[source] lock_spec_alt.
     Proof using MOD HAS_THREADS.
       verify_spec; ego.
+      wname [CustomMutexPreds.not_locked_ghost] "NL".
+      iFrame "NL". ego.
       Unshelve. all: exact (1$m)%cQp.
     Qed.
 
@@ -506,6 +558,8 @@ Module custom_mutex.
     Proof using MOD HAS_THREADS.
       verify_spec.
       repeat (go; ework).
+      wname [CustomMutexPreds.owner_token] "Owner".
+      iFrame "Owner". ego.
       Unshelve. all: exact (1$m)%cQp.
     Qed.
 
@@ -516,7 +570,7 @@ Module custom_mutex.
       wname [P] "P".
       wname [_ |-> atomic.R _ _ _] "L".
       wname [_ |-> thread_idR _ _] "Owner".
-      iMod (State.alloc 1%positive) as (gs) "(_ & T & State)".
+      iMod (alloc_state 1%positive) as (gs) "(_ & T & State)".
       iMod (cinv_alloc with "[L P Owner State]")
         as (gi) "[#CI CO]"; last first.
       - iModIntro. iExists (MkGname gs gi).
@@ -533,13 +587,13 @@ Module custom_mutex.
       work.
       wname [cinv] "#CI".
       wname [cinv_own] "CO".
-      wname [State.token] "T".
+      wname [CustomMutexPreds.token] "T".
       iMod (cinv_cancel with "CI CO")
         as "Inv"; [done..|].
       go.
       iDestruct "Inv" as (b) "(Lock & State & Resources)".
       destruct b.
-      - iDestruct (State.locked_full_token with "[$State $T]") as %[].
+      - iDestruct (locked_full_token with "[$State $T]") as %[].
       - iDestruct "Resources" as "[P Owner]".
         iAssert emp with "[State T]" as "_".
         { iApply (affine with "[State T]"); last iAccu. apply mpred_BiAffine. }
@@ -548,15 +602,13 @@ Module custom_mutex.
 
     Lemma mymutex_lock_proof : verify[source] lock_spec.
     Proof using MOD HAS_THREADS.
-      have -> : lock_spec ⊣⊢ lock_spec_alt.
-      { apply (Spec.lock_spec_equiv_lock_spec_alt IR lock_state_gname). done. }
+      rewrite lock_spec_equiv_lock_spec_alt.
       exact mymutex_lock_alt_proof.
     Qed.
 
     Lemma mymutex_unlock_proof : verify[source] unlock_spec.
     Proof using MOD HAS_THREADS.
-      have -> : unlock_spec ⊣⊢ unlock_spec_alt.
-      { apply (Spec.unlock_spec_equiv_unlock_spec_alt IR lock_state_gname). done. }
+      rewrite unlock_spec_equiv_unlock_spec_alt.
       exact mymutex_unlock_alt_proof.
     Qed.
 
