rocq-brick-libstdcpp/proof/mutex/spec/mutex.v
@@ -110,8 +110,11 @@ Module Type MUTEX_PREDS.
         { do_try_lock := do_try_lock }.
 
     (** Install [P] in an initialized mutex using its full representation and
-        token. The physical mutex remains initialized and unlocked. *)
-    Parameter install : forall (this : ptr) (old : gname)
+        token. The physical mutex remains initialized and unlocked.
+        
+        Initializing [this |-> R old 1$m emp] probably depends on the mutex
+        implementation. *)
+    Parameter init_R : forall (this : ptr) (old : gname)
         (pool : iprop.gname) (P : mpred),
       WeaklyObjective P ->
       this |-> R old 1$m emp ** token old 1$m ** ▷P |--
